Network_Security_Policy_Verification/TopoS_Helper.thy
@@ -5,7 +5,7 @@ imports Main TopoS_Interface
 begin
 
 lemma (in SecurityInvariant_preliminaries) sinvar_valid_remove_flattened_offending_flows:
-  assumes "wf_graph \<lparr>nodes = nodesG, edges = edgesG\<rparr>"
+  assumes "wf_graph \<lparr>nodes = nodesG, edges = edgesG\<rparr>" (*TODO: we could get rid of this assumption*)
   shows "sinvar \<lparr>nodes = nodesG, edges = edgesG - \<Union> (set_offending_flows \<lparr>nodes = nodesG, edges = edgesG\<rparr> nP) \<rparr> nP"
 proof -
   { fix f
@@ -19,6 +19,23 @@ proof -
   }
   with assms show ?thesis 
     by (metis (hide_lams, no_types) Diff_empty Union_empty defined_offending equals0I mono_sinvar wf_graph_remove_edges)
+qed
+
+
+lemma (in SecurityInvariant_preliminaries) sinvar_valid_remove_SOME_offending_flows:
+  assumes "set_offending_flows \<lparr>nodes = nodesG, edges = edgesG\<rparr> nP \<noteq> {}"
+  shows "sinvar \<lparr>nodes = nodesG, edges = edgesG - (SOME F. F \<in> set_offending_flows \<lparr>nodes = nodesG, edges = edgesG\<rparr> nP) \<rparr> nP"
+proof -
+  { fix f
+    assume *: "f\<in>set_offending_flows \<lparr>nodes = nodesG, edges = edgesG\<rparr> nP"
+
+    from * have 1: "sinvar \<lparr>nodes = nodesG, edges = edgesG - f \<rparr> nP"
+      by (metis (hide_lams, mono_tags) SecurityInvariant_withOffendingFlows.valid_without_offending_flows delete_edges_simp2 graph.select_convs(1) graph.select_convs(2))
+    from * have 2: "edgesG - \<Union> (set_offending_flows \<lparr>nodes = nodesG, edges = edgesG\<rparr> nP) \<subseteq> edgesG - f"
+      by blast
+    note 1 2
+  }
+  with assms show ?thesis by (simp add: some_in_eq)
 qed
 
 end
